theories/Block/vst/verif/certicoq_block__tag_is_noscan.v
@@ -1,0 +1,38 @@
+From VST Require Import floyd.proofauto.
+
+From CertiCoq Require Import Block.vst.ast.ast.
+From CertiCoq Require Import Block.vst.clightgen.block.
+From CertiCoq Require Import Block.vst.cmodel.certicoq_block_header.
+From CertiCoq Require Import Block.vst.cmodel.certicoq_block.
+From CertiCoq Require Import Block.vst.spec.spec.
+
+Lemma body: semax_body Vprog ASI f_certicoq_block__tag_is_noscan certicoq_block__tag_is_noscan_spec.
+Proof.
+  start_function.
+  forward_call.
+  forward_if.
+  {
+    forward.
+    entailer!.
+    destruct (block_tag_is_noscan_dec t) as [Hnoscan | Hnoscan] ; try reflexivity.
+    exfalso.
+    apply Hnoscan.
+    unfold block_tag_is_noscan.
+    apply negb_true_iff in H0.
+    apply lt_repr_false in H0 ; try assumption.
+    - admit.
+    - now split.
+  }
+  {
+    forward.
+    entailer!.
+    destruct (block_tag_is_noscan_dec t) as [Hnoscan | Hnoscan] ; try reflexivity.
+    exfalso.
+    apply negb_false_iff in H0.
+    apply lt_repr in H0.
+    - unfold block_tag_is_noscan in Hnoscan.
+      lia.
+    - admit.
+    - now split.
+  }
+Admitted.
